Wavelet/Compile/Fn/Simulation/Ret.lean
@@ -47,7 +47,7 @@ private theorem sim_step_ret_forwardc_sink
   simp [compileExpr] at hcurrent
   -- Step 1: Fire `forwardc`.
   have ⟨chans₁, retVals', hpop_ret_vals, hchans₁, hret_vals⟩ :=
-    pop_vals_singleton _ _
+    pop_vals_singleton
     (map := pc.chans)
     (names := vars.map (.var · gs.pathConds))
     (λ name val =>
@@ -102,7 +102,7 @@ private theorem sim_step_ret_forwardc_sink
   replace ⟨pc₁, hpc₁, hsteps₁⟩ := exists_eq_left.mpr hsteps₁
   -- Step 2: Fire `sink` to consume all unused channels in the current context.
   have ⟨chans₂, otherVals, hpop_other_vals, hchans₂, hother_vals⟩ :=
-    pop_vals_singleton _ _
+    pop_vals_singleton
     (map := pc₁.chans)
     (names := compileExpr.allVarsExcept gs.definedVars vars.toList gs.pathConds)
     (λ name val => True)
@@ -205,7 +205,7 @@ private theorem sim_step_ret_exec_dataflow
     := .step_tau hsteps₂.to_tau_star
   -- Step 4: Fire the `fork` in `compileFn`.
   simp only [compileFn, compileFn.resultSteers] at hcomp_fn
-  have ⟨chans₁, hpop_tail_cond, hchans₁⟩ := pop_val_singleton _ _
+  have ⟨chans₁, hpop_tail_cond, hchans₁⟩ := pop_val_singleton
     (map := intermChans m n gs vars
       (retValsToExprOutputs retVals)
       [])
@@ -228,13 +228,13 @@ private theorem sim_step_ret_exec_dataflow
   simp at hsteps₃
   replace ⟨pc₁, hpc₁, hsteps₃⟩ := exists_eq_left.mpr hsteps₃
   -- Step 5: Fire the first `steer` in `compileFn` for return values.
-  have ⟨chans₂, hpop_tail_cond_steer_dests, hchans₂⟩ := pop_val_singleton _ _
+  have ⟨chans₂, hpop_tail_cond_steer_dests, hchans₂⟩ := pop_val_singleton
     (map := pc₁.chans)
     (name := .tail_cond_steer_dests)
     (val := InterpConsts.fromBool false)
     (by simp [hpc₁, List.finIdxOf?, List.findFinIdx?, List.findFinIdx?.go])
   have ⟨chans₃, destVals, hpop_dest_vals, hchans₃, hdest_vals⟩ :=
-    pop_vals_singleton _ _
+    pop_vals_singleton
     (map := chans₂)
     (names := (Vector.range n).map (.dest · []))
     (λ name val =>
@@ -290,7 +290,7 @@ private theorem sim_step_ret_exec_dataflow
   simp at hsteps₄
   replace ⟨pc₂, hpc₂, hsteps₄⟩ := exists_eq_left.mpr hsteps₄
   -- Step 6: Fire the second `steer` in `compileFn` for tail call args.
-  have ⟨chans₄, hpop_tail_cond_steer_tail_args, hchans₄⟩ := pop_val_singleton _ _
+  have ⟨chans₄, hpop_tail_cond_steer_tail_args, hchans₄⟩ := pop_val_singleton
     (map := pc₂.chans)
     (name := .tail_cond_steer_tail_args)
     (val := InterpConsts.fromBool false)
@@ -298,7 +298,7 @@ private theorem sim_step_ret_exec_dataflow
       simp [hpc₂, hchans₃, hchans₂, hpc₁,
         List.finIdxOf?, List.findFinIdx?, List.findFinIdx?.go])
   have ⟨chans₅, tailArgVals, hpop_tail_arg_vals, hchans₅, htail_arg_vals⟩ :=
-    pop_vals_singleton _ _
+    pop_vals_singleton
     (map := chans₄)
     (names := (Vector.range m).map (.tail_arg · []))
     (λ name val => True)
@@ -330,7 +330,7 @@ private theorem sim_step_ret_exec_dataflow
   simp at hsteps₅
   replace ⟨pc₃, hpc₃, hsteps₅⟩ := exists_eq_left.mpr hsteps₅
   -- Step 7: Fire the first `carry` in `compileFn`.
-  have ⟨chans₆, hpop_tail_cond_steer_tail_args, hchans₆⟩ := pop_val_singleton _ _
+  have ⟨chans₆, hpop_tail_cond_steer_tail_args, hchans₆⟩ := pop_val_singleton
     (map := pc₃.chans)
     (name := .tail_cond_carry)
     (val := InterpConsts.fromBool false)
@@ -350,7 +350,7 @@ private theorem sim_step_ret_exec_dataflow
   simp at hsteps₆
   -- Step 8: Make the final transition to emit `.output` label
   have ⟨chans₇, destVals', hpop_final_dest_vals, hchans₇, hdest_vals⟩ :=
-    pop_vals_singleton _ _
+    pop_vals_singleton
     (map := chans₆)
     (names := (Vector.range n).map .final_dest)
     (λ name val =>
